project2/grep-naive/grep.dfy
@@ -6,9 +6,101 @@
  */
 
 include "Io.dfy"
+include "FileUtils.dfy"
+
+function method match_at(t: seq<byte>, p:seq<byte>, t_pos:nat): bool
+    requires 0 <= t_pos < |t|
+{
+    p <= t[t_pos..]
+}
+
+method first_match(t: seq<byte>, p:seq<byte>) returns (m: bool, n:nat)
+  requires |t| != 0
+  ensures m ==> 0 <= n < |t|
+  ensures !m ==> 0 <= n <= |t|
+  ensures m ==> match_at(t, p, n)
+  ensures forall k :: 0 <= k < n ==> !match_at(t, p, k)
+{
+  n := 0;
+  m := false;
+  while n < |t|
+    decreases |t| - n
+    invariant n <= |t|
+    invariant forall k :: 0 <= k < n ==> !match_at(t, p, k)
+  {
+    if match_at(t, p, n) {
+      m := true;
+      return;
+    }
+    n := n + 1;
+  }
+}
+
+method Grep(file: FileStream, length: int32, pattern: seq<byte>)
+  requires FileOk(file)
+  requires length as int == len(file)
+
+  modifies file
+  modifies file.env.ok
+  modifies file.env.files
+{
+  var ok, cont := ReadFile(file, length as nat32);
+  if (!ok) {
+    return;
+  }
+
+  if (|cont| == 0) {
+    print "NO\n";
+    return;
+  }
+
+  var m, n := first_match(cont, pattern);
+  if (m) {
+    print "YES: ";
+    print n;
+    print "\n";
+  } else {
+    print "NO\n";
+  }
+}
 
 method {:main} Main(ghost env:HostEnvironment?)
   requires env != null && env.Valid() && env.ok.ok();
+  modifies env.ok
+  modifies env.files
 {
-  print "TODO!\n";  
+  var num_args := HostConstants.NumCommandLineArgs(env);
+
+  if (num_args != 3) {
+    print "Expected usage: grep <file>\n";
+    return;
+  }
+
+  var pattern := HostConstants.GetCommandLineArg(1, env);
+  var source := HostConstants.GetCommandLineArg(2, env);
+  var source_exists := FileStream.FileExists(source, env);
+
+  if (!source_exists) {
+    print ("Source file does not exist.\n");
+    return;
+  }
+
+  var ok1, src_file := FileStream.Open(source, env);
+  if (!ok1) {
+    print "Error while opening source file.\n";
+    return;
+  }
+
+  var ok2, src_len := FileStream.FileLength(source, env);
+  if (!ok2) {
+    print "Error while opening source file.\n";
+    return;
+  }
+
+  Grep(src_file, src_len, seqa2seqb(pattern[..]));
+}
+
+function method {:verify false} seqa2seqb(s: seq<char>): seq<byte>
+{
+  if s == [] then [] else [s[0] as byte] + seqa2seqb(s[1..])
 }
